Work on adding delete and update to bags.

src/QueryStructure/Refinements/Bags/BagsInterface.v
@@ -2,6 +2,10 @@ Require Export Program Permutation.
 
 Unset Implicit Arguments.
 
+(* Enumerating the items of a Bag resulting from inserting
+   an item [inserted] into a bag [container] is a permutation
+   of adding [inserted] to the original set of elements.
+   *)
 Definition BagInsertEnumerate
            {TContainer TItem: Type}
            (benumerate : TContainer -> list TItem)
@@ -11,19 +15,16 @@ Definition BagInsertEnumerate
       (benumerate (binsert container inserted))
       (inserted :: benumerate container).
 
+(* The enumeration of an empty bag [bempty] is an empty list. *)
 Definition BagEnumerateEmpty
            {TContainer TItem: Type}
            (benumerate : TContainer -> list TItem)
            (bempty     : TContainer) :=
   forall item, ~ List.In item (benumerate bempty).
 
-Definition BagFindStar
-           {TContainer TItem TSearchTerm: Type}
-           (bfind : TContainer -> TSearchTerm -> list TItem)
-           (benumerate : TContainer -> list TItem)
-           (bstar : TSearchTerm) :=
-  forall container, bfind container bstar = benumerate container.
-
+(* [bfind] returns a permutation of the elements in a bag
+   [container] filtered by the match function [bfind_matcher]
+   using the specified search term [search_term]. *)
 Definition BagFindCorrect
            {TContainer TItem TSearchTerm: Type}
            (bfind         : TContainer -> TSearchTerm -> list TItem)
@@ -34,12 +35,53 @@ Definition BagFindCorrect
       (List.filter (bfind_matcher search_term) (benumerate container))
       (bfind container search_term).
 
+(* The [bstar] search term matches every item in a bag. *)
+Definition BagFindStar
+           {TContainer TItem TSearchTerm: Type}
+           (bfind : TContainer -> TSearchTerm -> list TItem)
+           (benumerate : TContainer -> list TItem)
+           (bstar : TSearchTerm) :=
+  forall container, bfind container bstar = benumerate container.
+
+(* [bcount] returns the number of elements in a bag which match
+   a search term [search_term]. *)
 Definition BagCountCorrect
            {TContainer TItem TSearchTerm: Type}
            (bcount        : TContainer -> TSearchTerm -> nat)
            (bfind         : TContainer -> TSearchTerm -> list TItem) :=
   forall container search_term,
     List.length (bfind container search_term) = (bcount container search_term).
+
+(* The elements of a bag [container] from which all elements matching
+   [search_term] have been deleted is a permutation of filtering
+   the enumeration of [container] by the negation of [search_term]. *)
+Definition BagDeleteCorrect
+           {TContainer TItem TSearchTerm: Type}
+           (bfind         : TContainer -> TSearchTerm -> list TItem)
+           (bfind_matcher : TSearchTerm -> TItem -> bool)
+           (benumerate : TContainer -> list TItem)
+           (bdelete    : TContainer -> TSearchTerm -> TContainer) :=
+  forall container search_term,
+    Permutation (benumerate (bdelete container search_term))
+                (snd (List.partition (bfind_matcher search_term)
+                                     (benumerate container))).
+
+(* The elements of a bag [container] in which the function [f_update]
+   has been applied to all elements matching [search_term]
+   is a permutation of partitioning the list into non-matching terms
+   and matching terms and mapping [f_update] over the latter. *)
+Definition BagUpdateCorrect
+           {TContainer TItem TSearchTerm: Type}
+           (bfind         : TContainer -> TSearchTerm -> list TItem)
+           (bfind_matcher : TSearchTerm -> TItem -> bool)
+           (benumerate : TContainer -> list TItem)
+           (bupdate    : TContainer -> TSearchTerm -> (TItem -> TItem) -> TContainer) :=
+  forall container search_term f_update,
+    Permutation (benumerate (bupdate container search_term f_update))
+                ((snd (List.partition (bfind_matcher search_term)
+                                      (benumerate container)))
+                   ++ List.map f_update (fst (List.partition (bfind_matcher search_term)
+                                                             (benumerate container)))).
 
 Class Bag (TContainer TItem TSearchTerm: Type) :=
   {
@@ -51,15 +93,19 @@ Class Bag (TContainer TItem TSearchTerm: Type) :=
     bfind      : TContainer -> TSearchTerm -> list TItem;
     binsert    : TContainer -> TItem -> TContainer;
     bcount     : TContainer -> TSearchTerm -> nat;
+    bdelete    : TContainer -> TSearchTerm -> TContainer;
+    bupdate    : TContainer -> TSearchTerm -> (TItem -> TItem) -> TContainer;
 
     binsert_enumerate : BagInsertEnumerate benumerate binsert;
     benumerate_empty  : BagEnumerateEmpty benumerate bempty;
     bfind_star        : BagFindStar bfind benumerate bstar;
     bfind_correct     : BagFindCorrect bfind bfind_matcher benumerate;
-    bcount_correct    : BagCountCorrect bcount bfind
+    bcount_correct    : BagCountCorrect bcount bfind;
+    bdelete_correct   : BagDeleteCorrect bfind bfind_matcher benumerate bdelete;
+    bupdate_correct   : BagUpdateCorrect bfind bfind_matcher benumerate bupdate
   }.
 
 Record BagPlusBagProof {TItem} :=
-  { BagType: Type; 
-    SearchTermType: Type; 
+  { BagType: Type;
+    SearchTermType: Type;
     BagProof: Bag BagType TItem SearchTermType }.
