src/QueryStructure/Refinements/Bags/CountingListBags.v
@@ -1,12 +1,27 @@
 Require Export BagsInterface.
 Unset Implicit Arguments.
 
-Record CountingList {A} := 
+Open Scope list.
+
+Record CountingList {A} :=
   {
     clength   : nat;
     ccontents : list A;
     cconsistent: List.length ccontents = clength
   }.
+
+Lemma empty_length {A} :
+  List.length (@nil A) = 0.
+Proof.
+  reflexivity.
+Qed.
+
+Definition CountingList_empty {TItem} : @CountingList TItem :=
+  {|
+    clength := 0;
+    ccontents := @nil TItem;
+    cconsistent := empty_length
+  |}.
 
 Fixpoint MatchAgainstMany {TItem}
          (search_terms : list (TItem -> bool)) (item: TItem) :=
@@ -15,7 +30,7 @@ Fixpoint MatchAgainstMany {TItem}
     | cons is_match more_terms => andb (is_match item) (MatchAgainstMany more_terms item)
   end.
 
-Definition CountingListAsBag_bfind 
+Definition CountingListAsBag_bfind
            {TItem: Type}
            (container: @CountingList TItem) (search_terms: list (TItem -> bool)) :=
   match search_terms with
@@ -30,9 +45,9 @@ Proof.
   intros; rewrite <- (cconsistent container); reflexivity.
 Qed.
 
-Definition CountingListAsBag_binsert 
+Definition CountingListAsBag_binsert
            {TItem: Type}
-           (container: @CountingList TItem) 
+           (container: @CountingList TItem)
            (item: TItem) : @CountingList TItem :=
   {| clength := S (clength container);
      ccontents := cons item (ccontents container);
@@ -43,9 +58,103 @@ Definition CountingListAsBag_bcount
            (container: @CountingList TItem) (search_terms: list (TItem -> bool)) :=
   match search_terms with
     | nil => clength container
-    | _   => List.fold_left (fun acc x => acc + if (MatchAgainstMany search_terms x) then 1 else 0) 
+    | _   => List.fold_left (fun acc x => acc + if (MatchAgainstMany search_terms x) then 1 else 0)
                             (ccontents container) 0
   end.
+
+Fixpoint CountingListPartition
+         {TItem: Type}
+         (contents : list TItem)
+         (search_term : TItem -> bool)
+: prod (@CountingList TItem) (@CountingList TItem) :=
+  match contents with
+    | nil => (CountingList_empty, CountingList_empty)
+    | x :: tl => let (g,d) := CountingListPartition tl search_term in
+                 if search_term x then
+                   (CountingListAsBag_binsert g x, d)
+                 else
+                   (g, CountingListAsBag_binsert d x)
+  end.
+
+Definition CountingListAsBag_bdelete
+           {TItem : Type}
+           (container : @CountingList TItem)
+           (search_terms : list (TItem -> bool)) :=
+  snd (CountingListPartition (ccontents container) (MatchAgainstMany search_terms)).
+
+Lemma CountingListMap_consistent
+      {TItem: Type}
+      (container: @CountingList TItem)
+      (update_f : TItem -> TItem)
+: length (List.map update_f (ccontents container)) = clength container.
+Proof.
+  rewrite List.map_length; auto using cconsistent.
+Qed.
+
+Definition CountingListMap
+         {TItem: Type}
+         (container: @CountingList TItem)
+         (update_f : TItem -> TItem)
+: @CountingList TItem :=
+  {| clength := clength container;
+     ccontents := List.map update_f (ccontents container);
+     cconsistent := CountingListMap_consistent container update_f|}.
+
+Lemma CountingListAsBag_Partition_App
+      {TItem : Type}
+      (container : @CountingList TItem)
+      (search_term : TItem -> bool)
+: length
+    (let (g, d) :=
+         CountingListPartition (ccontents container) search_term in
+     ccontents d ++ ccontents g) =
+  let (g, d) :=
+      CountingListPartition (ccontents container) search_term in
+  (clength g) + (clength d).
+Proof.
+  destruct container as [n l length_l]; simpl;
+  destruct (CountingListPartition l search_term); simpl.
+  rewrite List.app_length; repeat rewrite cconsistent; auto with arith.
+Qed.
+
+Lemma CountingListAsBag_bupdate_Consistent
+      {TItem : Type}
+      (container : @CountingList TItem)
+      (search_term : TItem -> bool)
+      (update_f : TItem -> TItem)
+: length
+    (let (g, d) :=
+         CountingListPartition (ccontents container) search_term in
+     ccontents d ++ List.map update_f (ccontents g)) =
+  clength container.
+Proof.
+  destruct container as [n l length_l]; simpl; revert n length_l;
+  induction l; simpl; intros; auto.
+  destruct (CountingListPartition l search_term); simpl.
+  erewrite <- length_l, <- (IHl (length l)); auto.
+  destruct (search_term a); simpl;
+  rewrite List.app_length; simpl; rewrite List.map_length;
+  repeat rewrite cconsistent; auto.
+  rewrite List.app_length; simpl; rewrite List.map_length;
+  repeat rewrite cconsistent; auto.
+Qed.
+
+Program Definition CountingListAsBag_bupdate
+           {TItem : Type}
+           (container : @CountingList TItem)
+           (search_terms : list (TItem -> bool))
+           (update_f : TItem -> TItem) :
+  @CountingList TItem :=
+  {| clength := clength container;
+     ccontents :=
+       let (g, d) := (CountingListPartition (ccontents container)
+                                            (MatchAgainstMany search_terms)) in
+       (ccontents d) ++ (List.map update_f (ccontents g));
+     cconsistent := CountingListAsBag_bupdate_Consistent
+                      container
+                      (MatchAgainstMany search_terms)
+                      update_f
+  |}.
 
 Lemma CountingList_BagInsertEnumerate :
   forall {TItem: Type},
@@ -54,26 +163,13 @@ Proof.
   firstorder.
 Qed.
 
-Lemma empty_length {A} :
-  List.length (@nil A) = 0.
-Proof.
-  reflexivity.
-Qed.
-
-Definition CountingList_empty {TItem} : @CountingList TItem :=
-  {| 
-    clength := 0;
-    ccontents := @nil TItem;
-    cconsistent := empty_length
-  |}.
-
 Lemma CountingList_BagEnumerateEmpty :
   forall {TItem: Type},
     BagEnumerateEmpty ccontents (@CountingList_empty TItem).
 Proof.
   firstorder.
 Qed.
-  
+
 Lemma CountingList_BagFindStar :
   forall {TItem: Type},
     BagFindStar (CountingListAsBag_bfind) (@ccontents TItem) nil.
@@ -97,14 +193,14 @@ Lemma CountingList_BagCountCorrect_aux :
     length (List.filter (MatchAgainstMany search_term) container) + default =
     List.fold_left
       (fun (acc : nat) (x : TItem) =>
-         acc + (if MatchAgainstMany search_term x then 1 else 0)) 
+         acc + (if MatchAgainstMany search_term x then 1 else 0))
       container default.
 Proof.
   induction container; intros.
 
   + trivial.
   + simpl; destruct (MatchAgainstMany search_term a);
-    simpl; rewrite <- IHcontainer; omega. 
+    simpl; rewrite <- IHcontainer; omega.
 Qed.
 
 Lemma CountingList_BagCountCorrect :
@@ -117,20 +213,56 @@ Proof.
   destruct search_term; simpl; [ apply cconsistent | apply temp ].
 Qed.
 
+Lemma CountingList_BagDeleteCorrect :
+  forall {TItem: Type},
+    BagDeleteCorrect (TItem := TItem) CountingListAsBag_bfind MatchAgainstMany ccontents
+                     CountingListAsBag_bdelete.
+Proof.
+  unfold BagDeleteCorrect; destruct container as [n l length_l];
+  revert n length_l; induction l; simpl; intros.
+  constructor.
+  pose proof (IHl _ (refl_equal _) search_term).
+  unfold CountingListAsBag_bdelete in *; simpl in *.
+  destruct (MatchAgainstMany search_term a);
+  destruct (CountingListPartition l (MatchAgainstMany search_term));
+  destruct (List.partition (MatchAgainstMany search_term) l); simpl; auto.
+Qed.
+
+Lemma CountingList_BagUpdateCorrect :
+  forall {TItem: Type},
+    BagUpdateCorrect (TItem := TItem) CountingListAsBag_bfind MatchAgainstMany ccontents
+                     CountingListAsBag_bupdate.
+Proof.
+  unfold BagUpdateCorrect; destruct container as [n l length_l];
+  revert n length_l; induction l; simpl; intros.
+  constructor.
+  pose proof (IHl _ (refl_equal _) search_term f_update).
+  unfold CountingListAsBag_bdelete in *; simpl in *.
+  destruct (MatchAgainstMany search_term a);
+  destruct (CountingListPartition l (MatchAgainstMany search_term));
+  destruct (List.partition (MatchAgainstMany search_term) l); simpl in *; auto.
+  rewrite Permutation_app_comm; simpl.
+  apply Permutation_cons_app; rewrite Permutation_app_comm; auto.
+Qed.
+
 Instance CountingListAsBag {TItem: Type}
 : Bag (@CountingList TItem) TItem (list (TItem -> bool)) :=
-  {| 
+  {|
     bempty := CountingList_empty;
     bstar  := nil;
-    
+
     benumerate := ccontents;
     bfind      := CountingListAsBag_bfind;
     binsert    := CountingListAsBag_binsert;
     bcount     := CountingListAsBag_bcount;
-    
+    bdelete    := CountingListAsBag_bdelete;
+    bupdate    := CountingListAsBag_bupdate;
+
     binsert_enumerate := CountingList_BagInsertEnumerate;
     benumerate_empty  := CountingList_BagEnumerateEmpty;
     bfind_star        := CountingList_BagFindStar;
     bfind_correct     := CountingList_BagFindCorrect;
-    bcount_correct    := CountingList_BagCountCorrect
+    bcount_correct    := CountingList_BagCountCorrect;
+    bdelete_correct     := CountingList_BagDeleteCorrect;
+    bupdate_correct     := CountingList_BagUpdateCorrect
   |}.
